## The Chain Rule: Case 1
Suppose that $z=f(x,y)$ is a differentiable function of $x$ and $y$, where $x=g(t)$ and $y=h(t)$ are both differentiable functions of $t$. Then $z$ is a differentiable function of $t$ and
$$\frac{dz}{dt}=\frac{\partial z}{\partial x}\frac{dx}{dt}+\frac{\partial z}{\partial y}\frac{dy}{dt}$$

### Proof
Since $z=f(x,y)$ is differentiable, we have
$$\Delta z=f_x(x_0,y_0)\Delta x+f_y(x_0,y_0)\Delta y+\varepsilon_1\Delta x+\varepsilon_2\Delta y$$
where $\varepsilon_1\to 0$ and $\varepsilon_2\to 0$ as $(\Delta x,\Delta y)\to (0,0)$. Dividing both sides by $\Delta t$, we have
$$\frac{\Delta z}{\Delta t}=\frac{\partial z}{\partial x}\frac{\Delta x}{\Delta t}+\frac{\partial z}{\partial y}\frac{\Delta y}{\Delta t}+\frac{\varepsilon_1}{\Delta t}\Delta x+\frac{\varepsilon_2}{\Delta t}\Delta y$$
If we let $\Delta t\to 0$, then $\Delta x=g(t+\Delta t)-g(t)\to 0$ because $g$ is differentiable and therefore continuous. Similarly, $\Delta y\to 0$. This, in turn, means that $\varepsilon_1\to 0$ and $\varepsilon_2\to 0$. Thus, we have
$$
\begin{aligned}
\frac{dz}{dt} &= \lim_{\Delta t\to 0}\frac{\Delta z}{\Delta t}\\
&= \frac{\partial f}{\partial x}\lim_{\Delta t\to 0}\frac{\Delta x}{\Delta t}+\frac{\partial f}{\partial y}\lim_{\Delta t\to 0}\frac{\Delta y}{\Delta t}+\left(\lim_{\Delta t\to 0}\varepsilon_1\right)\lim_{\Delta t\to 0}\frac{\Delta x}{\Delta t}+\left(\lim_{\Delta t\to 0}\varepsilon_2\right)\lim_{\Delta t\to 0}\frac{\Delta y}{\Delta t}\\
&= \frac{\partial f}{\partial x}\frac{dx}{dt}+\frac{\partial f}{\partial y}\frac{dy}{dt}+0\cdot \frac{dx}{dt}+0\cdot \frac{dy}{dt}\\
&= \frac{\partial f}{\partial x}\frac{dx}{dt}+\frac{\partial f}{\partial y}\frac{dy}{dt}
\end{aligned}
$$

## The Chain Rule: Case 2
Suppose that $z=f(x,y)$ is a differentiable function of $x$ and $y$, where $x=g(s,t)$ and $y=h(s,t)$ are differentiable functions of $s$ and $t$. Then
$$\frac{\partial z}{\partial s}=\frac{\partial z}{\partial x}\frac{\partial x}{\partial s}+\frac{\partial z}{\partial y}\frac{\partial y}{\partial s}$$
$$\frac{\partial z}{\partial t}=\frac{\partial z}{\partial x}\frac{\partial x}{\partial t}+\frac{\partial z}{\partial y}\frac{\partial y}{\partial t}$$

## The Chain Rule: General Version
Suppose that $u$ is a differentiable function of the $n$ variables $x_1,x_2,\dots,x_n$, and each $x_j$ is a differentiable function of the $m$ variables $t_1,t_2,\dots,t_m$. Then $u$ is a function of the $m$ variables $t_1,t_2,\dots,t_m$, and
$$\frac{\partial u}{\partial t_i}=\frac{\partial u}{\partial x_1}\frac{\partial x_1}{\partial t_i}+\frac{\partial u}{\partial x_2}\frac{\partial x_2}{\partial t_i}+\dots+\frac{\partial u}{\partial x_n}\frac{\partial x_n}{\partial t_i}$$
for each $i=1,2,\dots,m$.

## Implicit Differentiation
Suppose that an equation of the form $F(x,y)=0$ defines $y$ implicitly as a differentiable function of $x$, that is, $y=f(x)$, where $F(x,f(x))=0$ for all $x$ in the domain of $f$. If $F$ is differentiable, we can apply Case 1 of the Chain Rule to differentiate both sides of the equation $F(x,f(x))=0$ with respect to $x$. Since both $x$ and $y$ are functions of $x$, we obtain
$$\frac{\partial F}{\partial x}\frac{dx}{dx}+\frac{\partial F}{\partial y}\frac{dy}{dx}=0$$
But $\frac{dx}{dx}=1$, so if $\frac{\partial F}{\partial y}\neq 0$, we can solve for $\frac{dy}{dx}$ to obtain
$$\frac{dy}{dx}=-\frac{\frac{\partial F}{\partial x}}{\frac{\partial F}{\partial y}}=-\frac{F_x(x,y)}{F_y(x,y)}$$

For $F(x,y,z)=0$, we can apply the Chain Rule to differentiate both sides of the equation $F(x,y,z)=0$ with respect to $x$. We obtain
$$\frac{\partial F}{\partial x}\frac{\partial x}{\partial x}+\frac{\partial F}{\partial y}\frac{\partial y}{\partial x}+\frac{\partial F}{\partial z}\frac{\partial z}{\partial x}=0$$
Since we're differentiating with respect to $x$, $\frac{\partial y}{\partial x}=0$
Hence
$$\frac{\partial F}{\partial x}+\frac{\partial F}{\partial z}\frac{\partial z}{\partial x}=0$$
We can get
$$\frac{\partial z}{\partial x}=-\frac{\frac{\partial F}{\partial x}}{\frac{\partial F}{\partial z}}=-\frac{F_x}{F_z}$$
$$\frac{\partial z}{\partial y}=-\frac{\frac{\partial F}{\partial y}}{\frac{\partial F}{\partial z}}=-\frac{F_y}{F_z}$$